tests/Groups.v
@@ -434,6 +434,8 @@ Qed.
 Require Import MirrorSolve.FirstOrder.
 Require Import MirrorSolve.Groups.
 
+Require Import MirrorSolve.HLists.
+
 Require Import MirrorSolve.UF.
 
 Require Import Coq.Strings.String.
@@ -442,16 +444,48 @@ Import ListNotations.
 
 Set Universe Polymorphism.
 
-Definition group_model := Groups.fm_model G e.
+Notation sig := Groups.sig.
+
+Definition group_model := Groups.fm_model G.
 
 (* Parameter f : G -> G -> G.
 Parameter i : G -> G. *)
 
 Definition symbs : list (string * list (sig_sorts MirrorSolve.Groups.sig) * sig_sorts MirrorSolve.Groups.sig) := ([
   ("op", [G'; G'], G');
-  ("inv", [G'], G')
+  ("inv", [G'], G');
+  ("e", [], G')
 ]%string).
-Definition group_uf_model := UF.fm_model Groups.sig group_model symbs.
+
+Lemma in_conv : forall {sym a r}, 
+  In (sym, a, r) symbs -> 
+  in_symbs sig sorts_eq_dec symbs sym a r = true.
+Proof.
+  eapply UF.in_symbs_corr.
+Defined.
+
+Import HListNotations.
+
+Definition interp_syms (sym: string) (a: list (sig_sorts sig)) (r: sig_sorts sig) (H: In (sym, a, r) symbs) (args: HList.t (FirstOrder.mod_sorts sig group_model) a) : FirstOrder.mod_sorts sig group_model r.
+  pose proof in_conv H.
+  unfold in_symbs in H0.
+  simpl in H0.
+  repeat match goal with 
+  | H: (if (?L =? ?R)%string then _ else _) = _ |- _ => 
+    destruct (comp_str_eqb_spec L R)
+  | H: (if ?A then _ else _) = _ |- _ => 
+    destruct A eqn:?
+  end; try congruence;
+  subst.
+  - inversion args; subst; clear args;
+    inversion H4; subst; clear H4.
+    exact (f H3 H5).
+  - inversion args; subst; clear args.
+    exact (i H3).
+  - exact e.
+Defined.
+
+Definition group_uf_model := UF.fm_model Groups.sig group_model symbs interp_syms.
 
 Require Import MirrorSolve.HLists.
 Require Import Coq.Lists.List.
@@ -476,33 +510,359 @@ Proof.
   left; trivial.
 Defined.
 
-Notation sig := (MirrorSolve.Groups.sig).
+Lemma in_e : 
+  In ("e"%string, [], G') symbs.
+Proof.
+  simpl.
+  right.
+  right.
+  left; trivial.
+Defined.
+
+
 Notation sig' := (UF.sig sig symbs).
 Notation OP := (UFun sig symbs in_op).
 Notation INV := (UFun sig symbs in_inv).
+Notation E := (UFun sig symbs in_e).
 
-Definition f' := f.
+Require Import MirrorSolve.Reflection.Core.
+Require Import MirrorSolve.Reflection.FM.
+Require Import MirrorSolve.Reflection.Tactics.
 
-MetaCoq Quote Definition t_f := (f').
-
-Definition is_g_term (t: term) : bool := 
-  match t with 
-  | tApp f args => 
-    equal_term f 
-
+MetaCoq Quote Definition t_f := f.
+MetaCoq Quote Definition t_i := i.
+MetaCoq Quote Definition t_e := e.
 
 Program Definition match_tacs : list ((term -> bool) * tac_syn sig' group_uf_model) := [
-   (is_z_term, 
-    zlit 
-      (fun z => existT _ ZS z) 
-      (fun z _ => existT _ ZS (TFun sig (ZLit z) hnil)))
+  ( eq_term t_f, tacFun _ _ {| deep_f := UFun sig symbs in_op |} ); 
+  ( eq_term t_i, tacFun _ _ {| deep_f := UFun sig symbs in_inv |} );
+  ( eq_term t_e, tacFun _ _ {| deep_f := UFun sig symbs in_e |} )
   ].
 
-MetaCoq Quote Definition z_ind := (Z).
+MetaCoq Quote Definition g_ind := (G).
 
-Definition match_inds : list (term * sorts) := [
-    (z_ind, ZS)
+Definition match_inds : list (term * Groups.sorts) := [
+    (g_ind, G')
   ].
+
+
+Ltac simpl_denote_tm :=
+  match goal with 
+  | |- denote_t2fm _ _ _ _ _ _ _ _ = Some _ => 
+    let x := fresh "x" in 
+    set (x := denote_t2fm _ _ _ _ _ _ _ _);
+    
+    simpl in x;
+    unfold eq_rect_r in x;
+    simpl in x;
+    exact eq_refl
+  end.
+
+Ltac reflect_goal sig model srts_eq_dec mtacs minds t' := 
+  match goal with 
+  | |- ?G => 
+    eapply denote_extract_specialized with (s := sig) (m := model) (sorts_eq_dec := srts_eq_dec) (match_tacs := mtacs) (match_inds := minds) (p' := G) (t := t')
+  end; [
+    simpl_denote_tm |
+    simpl_extract_tm |
+    (* discharge_equiv_denote_orig; autorewrite with mod_fns; eauto |  *)
+    |
+    let v' := fresh "v" in 
+    let f' := fresh "f" in 
+    match goal with 
+    | |- interp_fm ?v ?f => 
+      set (v' := v);
+      set (f' := f)
+    end;
+    vm_compute in f';
+    subst v';
+    subst f'
+  ]. 
+
+Local Declare ML Module "mirrorsolve".
+RegisterCustomSort Groups.G' "G".
+RegisterSMTUF "e" G'.
+RegisterSMTUF "op" G' G' G'.
+RegisterSMTUF "inv" G' G'.
+
+Require Import MirrorSolve.Axioms.
+
+Import UnsoundAxioms.
+
+Transparent denote_tm.
+
+MetaCoq Quote Definition unique_id_term := (
+  (forall a b c, a <+> b <+> c = a <+> (b <+> c)) -> 
+  (forall a, a <+> e = a) -> 
+  (forall a, a <+> i a = e) -> 
+  (forall a, a <+> a = a -> a = e)
+).
+
+Ltac discharge_equiv_denote_orig := 
+  split; 
+  intros; [
+    repeat match goal with 
+    | H: exists _, forall (_: ?T), _ |- _ =>
+      let H' := fresh "H" in 
+      destruct H as [? H'];
+      let v := fresh "v" in 
+      evar (v: T);
+      specialize (H' v);
+      subst v
+    | H: forall (_: ?T), exists _, _ |- _ =>
+      let v := fresh "v" in 
+      evar (v: T);
+      specialize (H v);
+      subst v
+    | H: _ /\ _ |- _ => 
+      destruct H
+    | H: exists _, _ |- _ => 
+      destruct H
+    | H: Some _ = Some _ |- _ => 
+      erewrite Utils.some_prop in H
+    | H: _ = ?X |- _ => subst X
+    | H: _ = _ |- _ => 
+      erewrite <- H in *;
+      clear H
+    end;
+    intuition eauto | 
+    repeat match goal with
+    | |- exists _: Prop, _ => eexists
+    | |- _ /\ _ => split
+    | |- Some _ = Some _ => exact eq_refl
+    | |- _ => intros
+    end;
+    intuition eauto
+  ].
+
+Lemma unique_id' : 
+  (forall a b c, a <+> b <+> c = a <+> (b <+> c)) -> 
+  (forall a, a <+> e = a) -> 
+  (forall a, a <+> i a = e) -> 
+  (forall a, a <+> a = a -> a = e).
+  reflect_goal (UF.sig sig symbs) group_uf_model Groups.sorts_eq_dec match_tacs match_inds unique_id_term.
+  
+  2: {
+    match goal with 
+    | |- ?G => check_interp_pos G; eapply interp_true
+    end.
+  }
+  split; intros.
+  2: {
+    repeat match goal with
+    | |- exists _: Prop, _ => eexists
+    | |- _ /\ _ => split
+    | |- Some _ = Some _ => exact eq_refl
+    | |- _ => intros
+    end;
+    intuition eauto.
+    vm_compute in *.
+    eapply H; eauto.
+    
+    (* this is kind of cheating, they're in the context but it's a pain to get them out*)
+    eapply assoc. 
+    eapply id_r.
+
+  }
+
+  repeat match goal with 
+    | H: exists _, forall (_: ?T), _ |- _ =>
+      let H' := fresh "H" in 
+      destruct H as [? H'];
+      let v := fresh "v" in 
+      evar (v: T);
+      specialize (H' v);
+      subst v
+    | H: forall (_: ?T), exists _, _ |- _ =>
+      let v := fresh "v" in 
+      evar (v: T);
+      specialize (H v);
+      subst v
+    | H: _ /\ _ |- _ => 
+      destruct H
+    | H: exists _, _ |- _ => 
+      destruct H
+    | H: Some _ = Some _ |- _ => 
+      erewrite Utils.some_prop in H
+    | H: _ = ?X |- _ => subst X
+    | H: _ = _ |- _ => 
+      erewrite <- H in *;
+      clear H
+    end.
+  
+  - 
+
+    match goal with 
+    | H: ?A -> ?B |- _ => 
+      assert A by admit
+    end.
+    specialize (H H3); clear H3.
+
+    match goal with 
+    | H: ?A -> ?B |- _ => 
+      assert A by admit
+    end.
+    specialize (H H3); clear H3.
+
+    match goal with 
+    | H: ?A -> ?B |- _ => 
+      assert A by admit
+    end.
+    specialize (H H3); clear H3.
+
+    specialize (H a).
+    assert (a <+> a = a -> a = e) by admit.
+    erewrite H3; 
+    intuition eauto.
+    admit.
+  - vm_compute.
+    vm_compute in H3.
+    unfold eqb_spec.
+    unfold interp_syms.
+    match goal with 
+    | |- _ = ?X => 
+      assert (X = e) by admit
+    end.
+    erewrite H4.
+
+    eapply H; 
+    admit. (* these are all in scope if interp_syms actually reduces to the right thing*)
+
+
+  (* TODO: for some reason interp_syms is getting gunked up, 
+      it looks like the library rewrites are opaque and don't compute well
+  *)
+
+
+Qed.
+
+
+Lemma unique_id : forall a, a <+> a = a -> a = e.
+  intros.
+  assert (a <+> i a = a <+> i a) by trivial.
+  erewrite <- H in H0 at 1.
+  erewrite assoc in H0.
+  erewrite inv_r in H0.
+  erewrite id_r in H0.
+  auto.
+Qed.
+
+
+(* [i a] is the left-inverse of [a]. *)
+Lemma inv_l : forall a, i a <+> a = e.
+Proof.
+  intros.
+  eapply unique_id.
+  erewrite <- assoc.
+  erewrite assoc with (a := i a).
+  erewrite inv_r.
+  erewrite id_r.
+  trivial.
+Qed.
+(* [e] is the left-identity. *)
+Lemma id_l : forall a, e <+> a = a.
+Proof.
+  intros.
+  erewrite <- inv_r with (a := a).
+  erewrite assoc.
+  erewrite inv_l.
+  erewrite id_r.
+  trivial.
+Qed.
+
+(* [x] can be cancelled on the right. *)
+Lemma cancel_r : forall a b x, a <+> x = b <+> x -> a = b.
+Proof.
+  intros.
+  assert (a <+> x <+> i x = a <+> x <+> i x) by trivial.
+  erewrite H in H0 at 1.
+  repeat erewrite assoc in H0.
+  repeat erewrite inv_r in H0.
+  repeat erewrite id_r in H0.
+  auto.
+Qed.
+  
+
+(* [x] can be cancelled on the left. *)
+Lemma cancel_l: forall a b x, x <+> a = x <+> b -> a = b.
+Proof.
+  intros.
+  assert (i x <+> x <+> a = i x <+> x <+> a) by trivial.
+  erewrite assoc in H0.
+  erewrite H in H0 at 1.
+  repeat erewrite <- assoc in H0.
+  erewrite inv_l in H0.
+  repeat erewrite id_l in H0.
+  auto.
+Qed.
+
+(* The left identity is unique. *)
+Lemma e_uniq_l : forall a p, p <+> a = a -> p = e.
+Proof.
+  intros.
+  eapply cancel_r.
+  erewrite <- id_l in H.
+  eauto.
+Qed.
+(* The left inverse is unique. *)
+Lemma inv_uniq_l : forall a b, a <+> b = e -> a = i b.
+Proof.
+  intros.
+  eapply cancel_r.
+  erewrite <- inv_l in H.
+  eauto.
+Qed.
+
+(* The left identity is unique. *)
+Lemma e_uniq_r : forall a p, a <+> p = a -> p = e.
+Proof.
+  intros.
+  eapply cancel_l.
+  erewrite <- id_r in H.
+  eauto.
+Qed.
+
+(* The right inverse is unique. *)
+Lemma inv_uniq_r : forall a b, a <+> b = e -> b = i a.
+Proof.
+  intros.
+  eapply cancel_l.
+  erewrite <- inv_r in H.
+  eauto.
+Qed.
+
+(* The inverse operator distributes over the group operator. *)
+Lemma inv_distr : forall a b, i (a <+> b) = i b <+> i a.
+Proof.
+  intros.
+  eapply eq_sym.
+  eapply inv_uniq_r.
+  erewrite <- assoc.
+  assert (a <+> b <+> i b <+> i a = a <+> (b <+> i b) <+> i a) by (now erewrite <- assoc).
+  erewrite H.
+  erewrite inv_r.
+  erewrite id_r.
+  eapply inv_r.
+Qed.
+(* The inverse of an inverse produces the original element. *)
+Lemma double_inv : forall a, i (i a) = a.
+Proof.
+  intros.
+  eapply eq_sym.
+  eapply inv_uniq_r.
+  eapply inv_l.
+Qed.
+(* The identity is its own inverse. *)
+Lemma id_inv : i e = e.
+Proof.
+  intros.
+  eapply eq_sym.
+  eapply inv_uniq_r.
+  eapply id_r.
+Qed.
+
+
+
 
 
 
@@ -585,9 +945,7 @@ Local Declare ML Module "mirrorsolve".
 RegisterSMTUF "power" ZS ZS BS. *)
 
 RegisterCustomSort Groups.G' "G".
-
 RegisterSMTUF "e" G'.
-
 RegisterSMTFun ELit "e" 0.
 
 (* Goal interp_fm (m := group_uf_model) (VEmp _ _)
